Impl/QueryModel.i.dfy
@@ -28,70 +28,74 @@ module QueryModel {
   import opened BucketWeights
   import opened Bounds
   import opened BoundedPivotsLib
-
-  import PBS = PivotBetreeSpec`Internal
+  import opened TranslationLib
   import Messages = ValueMessage`Internal
 
   // == query ==
 
-  predicate queryInv(s: BBC.Variables, key: Key, msg: Message, ref: BT.G.Reference, io: IO, counter: uint64, lookup: seq<BT.G.ReadOp>)
+  predicate queryInv(s: BBC.Variables, querykey: Key, key: Key, msg: Message, ref: BT.G.Reference, 
+    io: IO, counter: int , lookup: seq<BT.Layer>)
   {
     && s.Ready?
     && BBC.Inv(s)
     && io.IOInit?
     && ref in s.ephemeralIndirectionTable.graph
     && counter >= 0
-    && (|lookup| == 0 ==> ref == BT.G.Root())
-    && (msg.Define? ==> |lookup| > 0)
-    && (|lookup| > 0 ==> BT.WFLookupForKey(lookup, key))
-    && (!msg.Define? ==> |lookup| > 0 ==> Last(lookup).node.children.Some?)
-    && (!msg.Define? ==> |lookup| > 0 ==> Last(lookup).node.children.value[Route(Last(lookup).node.pivotTable, key)] == ref)
-    && (forall i | 0 <= i < |lookup| :: lookup[i].ref in s.ephemeralIndirectionTable.graph)
-    && (forall i | 0 <= i < |lookup| :: MapsTo(s.cache, lookup[i].ref, lookup[i].node))
-    && (forall i | 0 <= i < |lookup| :: BoundedKey(lookup[i].node.pivotTable, key))
+    && (|lookup| == 0 ==> ref == BT.G.Root() && querykey == key)
+    && (msg.Define? ==> |lookup| > 0 && BT.WFLookupForKey(lookup, querykey))
+    && (!msg.Define? ==> |lookup| > 0 ==>
+        && BT.WFLookupForKey(lookup, querykey)
+        && Last(lookup).readOp.node.children.Some?
+        && Last(lookup).readOp.node.children.value[Route(Last(lookup).readOp.node.pivotTable, Last(lookup).currentKey)] == ref
+        && TranslateKey(Last(lookup).readOp.node.pivotTable, Last(lookup).readOp.node.edgeTable, Last(lookup).currentKey) == key)
+    && (forall i | 0 <= i < |lookup| :: lookup[i].readOp.ref in s.ephemeralIndirectionTable.graph)
+    && (forall i | 0 <= i < |lookup| :: MapsTo(s.cache, lookup[i].readOp.ref, lookup[i].readOp.node))
     && (ref in s.ephemeralIndirectionTable.graph)
-    && (PBS.LookupVisitsWellMarshalledBuckets(lookup, key) ==>
-        msg == BT.InterpretLookup(lookup, key))
+    && (BT.LookupVisitsWellMarshalledBuckets(lookup) ==> msg == BT.InterpretLookup(lookup))
   }
 
-
-  function {:opaque} new_lookup(lookup: seq<BT.G.ReadOp>, ref: BT.G.Reference, node: BT.G.Node) : seq<BT.G.ReadOp>
+  function new_lookup(lookup: seq<BT.Layer>, ref: BT.G.Reference, node: BT.G.Node, key: Key) : seq<BT.Layer>
   {
-    lookup + [BT.G.ReadOp(ref, node)]
+    lookup + [BT.Layer(BT.G.ReadOp(ref, node), key)]
   }
 
-  lemma AugmentLookup(lookup': seq<BT.G.ReadOp>, lookup: seq<BT.G.ReadOp>, ref: BT.G.Reference, node: BT.G.Node, key: Key, cache: map<BT.G.Reference, BT.G.Node>, graph: map<BT.G.Reference, seq<BT.G.Reference>>)
-  requires lookup' == new_lookup(lookup, ref, node)
-  requires |lookup| > 0 ==> BT.WFLookupForKey(lookup, key)
-  requires forall i | 0 <= i < |lookup| :: lookup[i].ref in graph
-  requires forall i | 0 <= i < |lookup| :: MapsTo(cache, lookup[i].ref, lookup[i].node)
-  requires forall i | 0 <= i < |lookup| :: BoundedKey(lookup[i].node.pivotTable, key)
-  requires |lookup| == 0 ==> ref == BT.G.Root()
-  requires |lookup| > 0 ==> Last(lookup).node.children.Some?
-  requires |lookup| > 0 ==> Last(lookup).node.children.value[Route(Last(lookup).node.pivotTable, key)] == ref
+  lemma AugmentLookup(lookup': seq<BT.Layer>, lookup: seq<BT.Layer>, querykey: Key, ref: BT.G.Reference, node: BT.G.Node, 
+    key: Key, cache: map<BT.G.Reference, BT.G.Node>, graph: map<BT.G.Reference, seq<BT.G.Reference>>)
+  requires lookup' == new_lookup(lookup, ref, node, key)
+  requires |lookup| == 0 ==> ref == BT.G.Root() && querykey == key
+  requires |lookup| > 0 ==>
+    && BT.WFLookupForKey(lookup, querykey)
+    && Last(lookup).readOp.node.children.Some?
+    && Last(lookup).readOp.node.children.value[Route(Last(lookup).readOp.node.pivotTable, Last(lookup).currentKey)] == ref
+    && TranslateKey(Last(lookup).readOp.node.pivotTable, Last(lookup).readOp.node.edgeTable, Last(lookup).currentKey) == key
+  requires forall i | 0 <= i < |lookup| :: lookup[i].readOp.ref in graph
+  requires forall i | 0 <= i < |lookup| :: MapsTo(cache, lookup[i].readOp.ref, lookup[i].readOp.node)
   requires BT.WFNode(node)
   requires MapsTo(cache, ref, node);
   requires BoundedKey(node.pivotTable, key)
-  requires ref in graph;
-  ensures BT.WFLookupForKey(lookup', key)
-  ensures Last(lookup').node == node
-  ensures BT.InterpretLookup(lookup', key) == Messages.Merge(BT.InterpretLookup(lookup, key), BT.NodeLookup(node, key))
-  ensures forall i | 0 <= i < |lookup'| :: lookup'[i].ref in graph
-  ensures forall i | 0 <= i < |lookup'| :: MapsTo(cache, lookup'[i].ref, lookup'[i].node)
-  ensures forall i | 0 <= i < |lookup'| :: BoundedKey(lookup'[i].node.pivotTable, key)
+  requires ref in graph
+  ensures |lookup'| > 0 && BT.WFLookupForKey(lookup', querykey)
+  ensures Last(lookup').readOp.node == node
+  ensures BT.InterpretLookup(lookup') == Messages.Merge(BT.InterpretLookup(lookup), BT.NodeLookup(node, key))
+  ensures forall i | 0 <= i < |lookup'| :: lookup'[i].readOp.ref in graph
+  ensures forall i | 0 <= i < |lookup'| :: MapsTo(cache, lookup'[i].readOp.ref, lookup'[i].readOp.node)
   {
-    reveal_new_lookup();
-
     forall idx | BT.ValidLayerIndex(lookup', idx) && idx < |lookup'| - 1
-    ensures BT.LookupFollowsChildRefAtLayer(key, lookup', idx)
+    ensures BT.LookupFollowsChildRefAtLayer(lookup', idx)
+    ensures BT.LookupFollowsChildEdgeAtLayer(lookup', idx)
     {
       if idx == |lookup'| - 2 {
-        assert BT.LookupFollowsChildRefAtLayer(key, lookup', idx);
+        assert BT.LookupFollowsChildRefAtLayer(lookup', idx);
+        assert BT.LookupFollowsChildEdgeAtLayer(lookup', idx);
       } else {
-        assert BT.LookupFollowsChildRefAtLayer(key, lookup, idx);
-        assert BT.LookupFollowsChildRefAtLayer(key, lookup', idx);
+        assert BT.LookupFollowsChildRefAtLayer(lookup, idx);
+        assert BT.LookupFollowsChildRefAtLayer(lookup', idx);
+
+        assert BT.LookupFollowsChildEdgeAtLayer(lookup, idx);
+        assert BT.LookupFollowsChildEdgeAtLayer(lookup', idx);
       }
     }
-    assert BT.LookupFollowsChildRefs(key, lookup');
+    assert BT.LookupFollowsChildRefs(lookup');
+    assert BT.LookupFollowsChildEdges(lookup');
   }
 }
