Impl/LeafImpl.i.dfy
@@ -56,16 +56,14 @@ module LeafImpl {
     if b {
       print "giving up; repivotLeaf can't run because frozen isn't written";
     } else {
-      var bounded := s.cache.NodeBoundedBucket(ref, ref, 0);
-      ghost var buckets := s.cache.I()[ref].buckets;
-      assert bounded == BoundedBucketList(buckets, s.cache.I()[ref].pivotTable);
-      if !bounded {
+      var _, edges, _ := s.cache.GetNodeInfo(ref);
+      if edges[0].Some? {
         print "giving up; repivotLeaf can't run because current leaf is incorrect";
       } else {
         var pivot: KeyType.Key;
         linear var left, right;
         var pivots := InitPivotTable();
-
+  
         left, right, pivot := s.cache.NodeSplitMiddle(ref);
         linear var buckets' := lseq_alloc(2);
         lseq_give_inout(inout buckets', 0, left);
@@ -74,7 +72,7 @@ module LeafImpl {
         pivot := CopyKey(pivot);
         pivots := Insert(pivots, Keyspace.Element(pivot), 1);
 
-        linear var newnode := Node(pivots, None, buckets');
+        linear var newnode := Node(pivots, [None, None], None, buckets');
         writeBookkeeping(inout s, ref, None);
         inout s.cache.Insert(ref, newnode);
         assert s.W();
@@ -82,7 +80,8 @@ module LeafImpl {
         ghost var a := s.I();
         ghost var oldnode := old_s.cache.I()[ref];
         ghost var b := LeafModel.repivotLeaf(old_s.I(), ref, oldnode);
-        assert newnode.I() == BT.G.Node(pivots, None, [
+        assert newnode.I() == BT.G.Node(pivots, [None, None], None, 
+            [
               SplitBucketLeft(oldnode.buckets[0], pivot),
               SplitBucketRight(oldnode.buckets[0], pivot)
             ]);
