Impl/SplitModel.i.dfy
@@ -21,17 +21,21 @@ module SplitModel {
   import opened KeyType
   import opened PivotBetreeSpec`Internal
   import opened BoundedPivotsLib
+  import opened TranslationLib
+  import opened TranslationImpl
   import PBSWF = PivotBetreeSpecWFNodes
 
   import opened NativeTypes
 
-  lemma lemmaChildrenConditionsCutoffNode(s: BBC.Variables, 
-      node: Node, lbound: Key, ubound: Option<Key>)
-  requires BT.WFNode(node)
+  lemma lemmaChildrenConditionsRestrictAndTranslateChild(s: BBC.Variables, 
+      parent: Node, child: Node, slot: int)
   requires s.Ready?
-  requires ValidSplitKey(node, lbound, ubound)
-  requires ChildrenConditions(s, node.children)
-  ensures ChildrenConditions(s, CutoffNode(node, lbound, ubound).children)
+  requires WFNode(parent)
+  requires WFNode(child)
+  requires 0 <= slot < NumBuckets(parent.pivotTable)
+  requires ParentKeysInChildRange(parent.pivotTable, parent.edgeTable, child.pivotTable, slot)
+  requires ChildrenConditions(s, child.children)
+  ensures ChildrenConditions(s, RestrictAndTranslateChild(parent, child, slot).children)
   {
     reveal_CutoffNode();
     reveal_CutoffNodeAndKeepLeft();
@@ -51,13 +55,14 @@ module SplitModel {
 
   // TODO can we get BetreeBlockCache to ensure that will be true generally whenever taking a betree step?
   // This sort of proof logic shouldn't have to be in the implementation.
-  lemma lemmaSplitChildValidReferences(child1: BT.G.Node, child: BT.G.Node, num_children_left: int, graph: map<BT.G.Reference, seq<BT.G.Reference>>, lbound: Key, ubound: Option<Key>)
+  lemma lemmaSplitChildValidReferences(parent: Node, child1: BT.G.Node, child: BT.G.Node, slot: int, num_children_left: int, graph: map<BT.G.Reference, seq<BT.G.Reference>>)
+  requires BT.WFNode(parent)
   requires BT.WFNode(child1)
-  requires BT.WFNode(child)
+  requires 0 <= slot < NumBuckets(parent.pivotTable)
+  requires ParentKeysInChildRange(parent.pivotTable, parent.edgeTable, child1.pivotTable, slot)
+  requires child == RestrictAndTranslateChild(parent, child1, slot)
   requires 1 <= num_children_left < |child.buckets|
-  requires ValidSplitKey(child1, lbound, ubound)
   requires BC.BlockPointsToValidReferences(child1, graph);
-  requires child == CutoffNode(child1, lbound, ubound);
   ensures BC.BlockPointsToValidReferences(BT.SplitChildLeft(child, num_children_left), graph);
   ensures BC.BlockPointsToValidReferences(BT.SplitChildRight(child, num_children_left), graph);
   {
@@ -103,14 +108,12 @@ module SplitModel {
   requires ChildrenConditions(s, right_child.children)
   requires ChildrenConditions(s, Some(fused_parent_children))
   requires |fused_parent_children| < MaxNumChildren()
-  // requires |s.ephemeralIndirectionTable.graph| <= IT.MaxSize() - 3
   ensures s'.Ready?
   ensures s'.cache == s.cache
   {
     lemmaChildrenConditionsPreservedWriteBookkeeping(s, left_childref, left_child.children, right_child.children);
     lemmaChildrenConditionsPreservedWriteBookkeeping(s, left_childref, left_child.children, Some(fused_parent_children));
     lemmaRefInGraphOfWriteBookkeeping(s, left_childref, left_child.children);
-
     var s1 := writeBookkeeping(s, left_childref, left_child.children);
 
     lemmaChildrenConditionsPreservedWriteBookkeeping(s1, right_childref, right_child.children, Some(fused_parent_children));
@@ -131,7 +134,6 @@ module SplitModel {
   requires s.Ready?
   requires parentref in s.cache
   requires BT.WFNode(s.cache[parentref]);
-  requires PivotInsertable(s.cache[parentref].pivotTable, slot+1, pivot)
   requires s.cache[parentref].children.Some?
   requires 0 <= slot < |s.cache[parentref].children.value|
   {
@@ -148,8 +150,11 @@ module SplitModel {
       fused_parent_children: seq<BT.G.Reference>, slot: int) : (s': BBC.Variables)
   requires s.Ready?
   requires parentref in s.cache
-  requires BT.WFNode(s.cache[parentref]);
-  requires BT.WFNode(child);
+  requires WFNode(s.cache[parentref]);
+  requires WFPivots(child.pivotTable)
+  requires NumBuckets(child.pivotTable) == |child.buckets|
+  requires |child.edgeTable| == |child.buckets| 
+  requires child.children.Some? ==> |child.children.value| == |child.buckets|
   requires s.cache[parentref].children.Some?
   requires 0 <= slot < |s.cache[parentref].children.value|
   requires 0 <= slot < |fused_parent_children|
@@ -158,64 +163,20 @@ module SplitModel {
   requires ChildrenConditions(s, Some(fused_parent_children))
   requires ChildrenConditions(s, child.children)
   requires |fused_parent_children| < MaxNumChildren()
-  // requires |s.ephemeralIndirectionTable.graph| <= IT.MaxSize() - 3
   {
     var num_children_left := |child.buckets| / 2;
     var pivot := GetKey(child.pivotTable, num_children_left);
 
-    if PivotInsertable(s.cache[parentref].pivotTable, slot+1, pivot) then (
-      lemmaChildrenConditionsSplitChild(s, child, num_children_left);
-
-
+    if !PivotInsertable(s.cache[parentref].pivotTable, slot+1, pivot) then (
+      s
+    ) else if !SplitChildrenWeight(child.buckets, num_children_left) then (
+      s
+    ) else (
       var left_child := SplitChildLeft(child, num_children_left);
       var right_child := SplitChildRight(child, num_children_left);
       var s3 := splitBookkeeping(s, left_childref, right_childref, parentref, fused_parent_children, left_child, right_child, slot);
       var s' := splitCacheChanges(s3, left_childref, right_childref, parentref, slot, num_children_left, pivot, left_child, right_child);
       s'
-    ) else (
-      s
-    )
-  }
-
-  function {:opaque} splitChild(s: BBC.Variables, parentref: BT.G.Reference, 
-    childref: BT.G.Reference, slot: int, lbound: Key, ubound: Option<Key>, refUpperBound: uint64): (s': BBC.Variables)
-  requires s.Ready?
-  requires BBC.Inv(s)
-  requires parentref in s.cache
-  requires childref in s.cache
-  requires BT.WFNode(s.cache[parentref]);
-  requires BT.WFNode(s.cache[childref]);
-  requires s.cache[parentref].children.Some?
-  requires 0 <= slot < |s.cache[parentref].children.value|
-  requires s.cache[parentref].children.value[slot] == childref
-  requires ValidSplitKey(s.cache[childref], lbound, ubound)
-  requires ChildrenConditions(s, s.cache[childref].children)
-  requires ChildrenConditions(s, s.cache[parentref].children)
-  requires |s.cache[parentref].children.value| < MaxNumChildren()
-  requires forall r | r in s.ephemeralIndirectionTable.graph :: r <= refUpperBound
-  {
-    var fused_parent := s.cache[parentref];
-    var fused_child := s.cache[childref];
-
-    var child := CutoffNode(fused_child, lbound, ubound);
-    lemmaChildrenConditionsCutoffNode(s, fused_child, lbound, ubound);
-    if (|child.pivotTable| == 2) then (
-      // TODO there should be an operation which just
-      // cuts off the node and doesn't split it.
-      s
-    ) else (
-      var left_childref := getFreeRef(s, refUpperBound);
-      if left_childref.None? then (
-        s
-      ) else (
-        var right_childref := getFreeRef2(s, left_childref.value, refUpperBound);
-        if right_childref.None? then (
-          s
-        ) else (
-          splitDoChanges(s, child, left_childref.value, right_childref.value,
-            parentref, fused_parent.children.value, slot)
-        )
-      )
     )
   }
 
@@ -242,23 +203,36 @@ module SplitModel {
       var fused_parent := s.cache[parentref];
       var fused_child := s.cache[childref];
 
-      if !( 
-        && Keyspace.lte(fused_child.pivotTable[0], fused_parent.pivotTable[slot])
-        && Keyspace.lte(fused_parent.pivotTable[slot+1], Last(fused_child.pivotTable))
+      if !( ParentKeysInChildRange(fused_parent.pivotTable, fused_parent.edgeTable, fused_child.pivotTable, slot)
       ) then (
         s
       ) else (
-        lemmaChildrenConditionsOfNode(s, parentref);
-        lemmaChildrenConditionsOfNode(s, childref);
+        var lcp := PivotLcp(fused_parent.pivotTable[slot], fused_parent.pivotTable[slot+1]);
+        var prefix := fused_parent.edgeTable[slot];
+        if ( prefix.None? || (prefix.Some? && TranslateBucketsWillFit(fused_child.buckets, prefix.value, lcp))) then (
+          lemmaChildrenConditionsOfNode(s, parentref);
+          lemmaChildrenConditionsOfNode(s, childref);
 
-        var lbound := getlbound(fused_parent, slot);
-        var ubound := getubound(fused_parent, slot);
-
-        if (
-          && ValidSplitKey(fused_child, lbound, ubound) 
-          && ValidSplitKey(fused_parent, lbound, ubound)
-        ) then (
-          splitChild(s, parentref, childref, slot, lbound, ubound, refUpperBound)
+          var child := RestrictAndTranslateChild(fused_parent, fused_child, slot);
+          if (|child.pivotTable| == 2) then (
+            // TODO there should be an operation which just
+            // cuts off the node and doesn't split it.
+            s
+          ) else (
+            lemmaChildrenConditionsRestrictAndTranslateChild(s, fused_parent, fused_child, slot);
+            var left_childref := getFreeRef(s, refUpperBound);
+            if left_childref.None? then (
+              s
+            ) else (
+              var right_childref := getFreeRef2(s, left_childref.value, refUpperBound);
+              if right_childref.None? then (
+                s
+              ) else (
+                splitDoChanges(s, child, left_childref.value, right_childref.value,
+                  parentref, fused_parent.children.value, slot)
+              )
+            )
+          )
         ) else (
           s
         )
@@ -284,13 +258,19 @@ module SplitModel {
     ) {
       assert noop(s, s);
       return;
-    } 
+    }
+
     var fused_parent := s.cache[parentref];
     var fused_child := s.cache[childref];
-    if !( 
-        && Keyspace.lte(fused_child.pivotTable[0], fused_parent.pivotTable[slot])
-        && Keyspace.lte(fused_parent.pivotTable[slot+1], Last(fused_child.pivotTable))
-    ) {
+
+    if !( ParentKeysInChildRange(fused_parent.pivotTable, fused_parent.edgeTable, fused_child.pivotTable, slot)) {
+      assert noop(s, s);
+      return;
+    }
+
+    var lcp := PivotLcp(fused_parent.pivotTable[slot], fused_parent.pivotTable[slot+1]);
+    var prefix := fused_parent.edgeTable[slot];
+    if !(prefix.None? || (prefix.Some? && TranslateBucketsWillFit(fused_child.buckets, prefix.value, lcp))) {
       assert noop(s, s);
       return;
     }
@@ -298,28 +278,15 @@ module SplitModel {
     lemmaChildrenConditionsOfNode(s, parentref);
     lemmaChildrenConditionsOfNode(s, childref);
 
-    var lbound := getlbound(fused_parent, slot);
-    var ubound := getubound(fused_parent, slot);
-
-    if !(
-      && ValidSplitKey(fused_child, lbound, ubound) 
-      && ValidSplitKey(fused_parent, lbound, ubound)
-    ) {
-      assert noop(s, s);
-      return;
-    }
-
-    reveal_splitChild();
-    var child := CutoffNode(fused_child, lbound, ubound);
-    lemmaChildrenConditionsCutoffNode(s, fused_child, lbound, ubound);
-
+    var child := RestrictAndTranslateChild(fused_parent, fused_child, slot);
     if (|child.pivotTable| == 2) {
       // TODO there should be an operation which just
-      // cuts off the node and doesn't split it.          
+      // cuts off the node and doesn't split it.
       assert noop(s, s);
       return;
     }
 
+    lemmaChildrenConditionsRestrictAndTranslateChild(s, fused_parent, fused_child, slot);
     var left_childref := getFreeRef(s, refUpperBound);
     if left_childref.None? {
       assert noop(s, s);
@@ -340,7 +307,12 @@ module SplitModel {
       assert noop(s, s);
       return;
     }
-      
+
+    if !SplitChildrenWeight(child.buckets, num_children_left) {
+      assert noop(s, s);
+      return;
+    }
+ 
     lemmaChildrenConditionsSplitChild(s, child, num_children_left);
     var left_child := SplitChildLeft(child, num_children_left);
     var right_child := SplitChildRight(child, num_children_left);
@@ -380,7 +352,7 @@ module SplitModel {
     PBSWF.ValidSplitWritesWFNodes(splitStep);
     lemmaBlockPointsToValidReferences(s, childref);
     assert BC.BlockPointsToValidReferences(fused_child, s.ephemeralIndirectionTable.graph);
-    lemmaSplitChildValidReferences(fused_child, child, num_children_left, s.ephemeralIndirectionTable.graph, lbound, ubound);
+    lemmaSplitChildValidReferences(fused_parent, fused_child, child, slot, num_children_left, s.ephemeralIndirectionTable.graph);
 
     writeNewRefIsAlloc(s, left_childref.value, left_child);
     writeNewRefIsAlloc(s1, right_childref.value, right_child);
@@ -389,9 +361,7 @@ module SplitModel {
     assert BC.BlockPointsToValidReferences(fused_parent, s2.ephemeralIndirectionTable.graph);
     lemmaSplitParentValidReferences(fused_parent, pivot, slot, left_childref.value, right_childref.value, s2.ephemeralIndirectionTable.graph);
 
-    assert child == CutoffNode(fused_child, lbound, ubound);
     assert 1 <= num_children_left < |child.buckets|;
-
     assert splitStep.num_children_left == num_children_left;
     assert splitStep.fused_child == fused_child;
     assert left_childref.value != right_childref.value;
