lib/Buckets/TranslationImpl.i.dfy
@@ -1,0 +1,833 @@
+include "BoundedPivotsLib.i.dfy"
+include "TranslationLib.i.dfy"
+include "BucketImpl.i.dfy"
+
+include "../Base/KeyType.s.dfy"
+include "../Lang/LinearSequence.i.dfy"
+include "../Lang/LinearSequence.s.dfy"
+
+//
+// Provides definitions and libraries for edge table and 
+// other translation related methods and lemma
+//
+
+module TranslationImpl {
+  import opened NativeTypes
+  import opened BoundedPivotsLib
+  import opened Translations = TranslationLib
+  import opened Sequences
+  import opened Options
+  import opened KeyType
+  import opened ValueMessage
+  import opened BucketImpl
+  import opened BucketsLib
+  import opened LinearSequence_i
+  import opened LinearSequence_s
+
+  method ComputeSplitLeftEdges(et: EdgeTable, pt: PivotTable, pt': PivotTable, pivot: Key, cLeft: uint64) returns (et': EdgeTable)
+  requires WFPivots(pt)
+  requires WFEdges(et, pt)
+  requires ValidLeftCutOffKey(pt, pivot)
+  requires |pt| < 0x4000_0000_0000_0000
+  requires cLeft as int == CutoffForLeft(pt, pivot)
+  requires pt' == SplitLeft(pt, pivot)
+  ensures et' == SplitLeftEdges(et, pt, pivot)
+  {
+    if (pt[cLeft + 1].Element? && pt[ cLeft+1 ].e == pivot) || et[cLeft].None? {
+      return et[..cLeft + 1];
+    } else {
+      var oldlcp : Key := ComputePivotLcp(pt[cLeft], pt[cLeft+1]);
+      var newlcp : Key := ComputePivotLcp(pt'[cLeft], pt'[cLeft+1]);
+      PivotLcpSubRangeLeft(pt[cLeft], pt[cLeft+1], pt'[cLeft+1]);
+
+      assume |et[cLeft].value + newlcp[|oldlcp|..]| <= 1024;
+      var translation : Key := et[cLeft].value + newlcp[|oldlcp|..];
+      return et[..cLeft] +  [Some(translation)];
+    }
+  }
+
+  method ComputeSplitRightEdges(et: EdgeTable, pt: PivotTable, pt': PivotTable, pivot: Key, cRight: uint64) returns (et': EdgeTable)
+  requires WFPivots(pt)
+  requires WFEdges(et, pt)
+  requires BoundedKey(pt, pivot)
+  requires |pt| < 0x4000_0000_0000_0000
+  requires cRight as int == CutoffForRight(pt, pivot)
+  requires pt' == SplitRight(pt, pivot)
+  ensures et' == SplitRightEdges(et, pt, pivot)
+  {
+    if pt[cRight].e == pivot || et[cRight].None? {
+      return et[cRight..];
+    } else {
+      var oldlcp : Key := ComputePivotLcp(pt[cRight], pt[cRight+1]);
+      var newlcp : Key := ComputePivotLcp(pt'[0], pt'[1]);
+      PivotLcpSubRangeRight(pt[cRight], pt'[0], pt'[1]);
+
+      assume |et[cRight].value + newlcp[|oldlcp|..]| <= 1024;
+      var translation : Key := et[cRight].value + newlcp[|oldlcp|..];
+      return [Some(translation)] + et[cRight+1..];
+    }
+  }
+
+  lemma lcprightCondition(s: Key, len: nat)
+    requires len <= |s|
+    requires forall j | 0 <= j < len :: s[j] == 255
+    requires len == |s| || s[len] < 255
+    ensures s[..len] == lcpright(s)
+  {
+    if |s| == 0 || s[0] < 255 {
+    } else {
+      lcprightCondition(s[1..], len-1);
+    }
+  }
+
+  method ComputelcprightLen(left: Key) returns (len: uint64)
+  ensures len as nat == |lcpright(left)|
+  {
+    var i: uint64 := 0;
+    var llen := |left| as uint64;
+
+    while i < llen && left[i] == 255
+      invariant 0 <= i <= llen
+      invariant forall j | 0 <= j < i :: left[j] as int == Uint8UpperBound() as int - 1
+    {
+      i := i + 1;
+    }
+    lcprightCondition(left, i as nat);
+    return i;
+  }
+
+  method Computelcpright(left: Key) returns (prefix: Key)
+  ensures prefix == lcpright(left)
+  {
+    var len := ComputelcprightLen(left);
+    return left[..len];
+  }
+
+  lemma lcpCondition(left: Key, right: Key, common_len: nat)
+    requires common_len <= |left|
+    requires common_len <= |right|
+    requires forall j | 0 <= j < common_len :: left[j] == right[j]
+    requires common_len == |left| || common_len == |right| || left[common_len] != right[common_len]
+    ensures lcp(left, right) ==
+      if common_len < |left| && common_len + 1 == |right| && left[common_len] as nat + 1 == right[common_len] as nat then
+        left[..common_len + 1] + lcpright(left[common_len + 1..])
+      else
+        left[..common_len]
+  {
+    if 0 < common_len {
+      lcpCondition(left[1..], right[1..], common_len-1);
+    }
+  }
+
+  method ComputelcpLen(left: Key, right: Key) returns (len: uint64)
+  ensures len as nat == |lcp(left, right)|
+  {
+    var i: uint64 := 0;
+    while
+      && i < |left| as uint64
+      && i < |right| as uint64
+      && left[i] == right[i]
+      invariant i as nat <= |left|
+      invariant i as nat <= |right|
+      invariant forall j | j < i :: left[j] == right[j]
+    {
+      i := i + 1;
+    }
+    lcpCondition(left, right, i as nat);
+
+    if
+      && i < |left| as uint64
+      && i + 1 == |right| as uint64
+      && left[i] < right[i]
+      && left[i] + 1 == right[i] {
+        i := i + 1;
+        ghost var s := i;
+        while
+          && i < |left| as uint64
+          && left[i] == 255
+          invariant s as nat <= i as nat <= |left|
+          invariant forall j | s <= j < i :: left[j] == 255
+        {
+          i := i + 1;
+        }
+        lcprightCondition(left[s..], i as nat - s as nat);
+    }
+    len := i;
+  }
+
+  method Computelcp(left: Key, right: Key) returns (prefix: Key)
+  ensures prefix == lcp(left, right)
+  {
+    var len := ComputelcpLen(left, right);
+    prefix := left[..len];
+  }
+
+  method ComputePivotLcpLen(left: Element, right: Element) returns (len: uint64)
+  requires ElementIsKey(left)
+  requires right.Element? ==> ElementIsKey(right)
+  ensures len as nat == |PivotLcp(left, right)|
+  {
+    if right.Max_Element? {
+      len := ComputelcprightLen(left.e);
+    } else {
+      len := ComputelcpLen(left.e, right.e);
+    }
+  }
+
+  method ComputePivotLcp(left: Element, right: Element) returns (prefix: Key)
+  requires ElementIsKey(left)
+  requires right.Element? ==> ElementIsKey(right)
+  ensures prefix == PivotLcp(left, right)
+  {
+    var len := ComputePivotLcpLen(left, right);
+    prefix := left.e[..len];
+  }
+
+  method ComputeTranslatePrefixSet(pt: PivotTable, et: EdgeTable, key: Key, r: uint64) returns (pset: Option<PrefixSet>)
+  requires |pt| < 0x4000_0000_0000_0000
+  requires WFPivots(pt)
+  requires BoundedKey(pt, key)
+  requires WFEdges(et, pt)
+  requires r as int == Route(pt, key)
+  ensures pset == Translate(pt, et, key)
+  {
+    if et[r].Some? {
+      var prefixlen := ComputePivotLcpLen(pt[r], pt[r+1]);
+      PrefixOfLcpIsPrefixOfKey(pt[r], pt[r+1], pt[r].e[..prefixlen], key);
+      pset := Some(PrefixSet(pt[r].e[..prefixlen], et[r].value));
+    } else {
+      pset := None;
+    }
+  }
+
+  method ComputeTranslateKey(pt: PivotTable, et: EdgeTable, key: Key, r: uint64) returns (k: Key)
+  requires |pt| < 0x4000_0000_0000_0000
+  requires WFPivots(pt)
+  requires BoundedKey(pt, key)
+  requires WFEdges(et, pt)
+  requires r as int == Route(pt, key)
+  ensures k == TranslateKey(pt, et, key)
+  {
+    if et[r].Some? {
+      var prefixlen := ComputePivotLcpLen(pt[r], pt[r+1]);
+      PrefixOfLcpIsPrefixOfKey(pt[r], pt[r+1], pt[r].e[..prefixlen], key);
+      assume |et[r].value| + |key| - prefixlen as nat <= 1024;
+      k := et[r].value + key[prefixlen..];
+    } else {
+      k := key;
+    }
+  }
+
+  method ComputeComposePrefixSet(a: Option<PrefixSet>, b: Option<PrefixSet>) returns (c: Option<PrefixSet>)
+  requires ComposePrefixSet.requires(a, b)
+  ensures c == ComposePrefixSet(a, b)
+  {
+    if b.None? {
+      c := a;
+    } else if a.None? {
+      c := Some(PrefixSet(b.value.newPrefix, b.value.prefix));
+    } else if |a.value.prefix| as uint64 <= |b.value.prefix| as uint64 {
+      reveal_IsPrefix();
+      var newPrefix := ApplyPrefixSet(a, b.value.prefix);
+      c := Some(PrefixSet(b.value.newPrefix, newPrefix));
+    } else {
+      var prefix := ApplyPrefixSet(b, a.value.prefix);
+      c := Some(PrefixSet(prefix, a.value.newPrefix));
+    }
+  }
+
+  method ComputeShortestUncommonPrefix(prefix: Key) returns (upper: Element)
+  ensures upper == ShortestUncommonPrefix(prefix, |prefix|)
+  {
+    reveal_ShortestUncommonPrefix();
+    var i: int64 := |prefix| as int64 - 1;
+    while 0 <= i && prefix[i] == 255
+      invariant -1 <= i as int < |prefix|
+      invariant forall j | i as int < j < |prefix| :: prefix[j] == 255
+      invariant ShortestUncommonPrefix(prefix, |prefix|) == ShortestUncommonPrefix(prefix, i as int + 1)
+    {
+      i := i - 1;
+    }
+    if i == -1 {
+      upper := Keyspace.Max_Element;
+    } else {
+      var c := prefix[i] + 1;
+      upper := Keyspace.Element(prefix[..i] + [c]);
+    }
+  }
+
+  method ComputeTranslateElement(e: Element, prefix: Key, newPrefix: Key) returns (e': Element)
+  requires ElementIsKey(e)
+  requires IsPrefix(prefix, e.e)
+  ensures e' == TranslateElement(e, prefix, newPrefix)
+  {
+    e' := Keyspace.Element(newPrefix + e.e[|prefix| as uint64..]);
+  }
+
+  method ComputeTranslatePivotPair(left: Key, right: Element, prefix: Key, newPrefix: Key)
+  returns (left': Key, right': Element)
+  requires right.Element? ==> ElementIsKey(right)
+  requires IsPrefix(prefix, left)
+  requires Keyspace.lt(KeyToElement(left), right)
+  ensures var (l, r) := TranslatePivotPairInternal(KeyToElement(left), right, prefix, newPrefix);
+    && l == KeyToElement(left')
+    && r == right'
+  {
+    assume |newPrefix + left[|prefix|..]| <= 1024;
+    left' := newPrefix + left[|prefix| as uint64..];
+    // left' := ComputeTranslateElement(left, prefix, newPrefix);
+
+    var isprefix := right.Element? && |prefix| as uint64 <= |right.e| as uint64 && prefix == right.e[..|prefix|];
+    reveal_IsPrefix();
+    if right.Max_Element? || !isprefix {
+      right' := ComputeShortestUncommonPrefix(newPrefix);
+    } else {
+      right' := ComputeTranslateElement(right, prefix, newPrefix);
+    }
+  }
+
+  lemma TranslatePivotsCondition(pt: PivotTable, prefix: Key, newPrefix: Key, end: Element, idx: nat, pt': PivotTable)
+    requires TranslatePivots.requires(pt, prefix, newPrefix, end, idx)
+    requires |pt'| == |pt| - idx
+    requires forall i | 0 <= i < |pt'| - 1 :: pt'[i] == TranslateElement(pt[idx + i], prefix, newPrefix)
+    requires Last(pt') == end
+    ensures pt' == TranslatePivots(pt, prefix, newPrefix, end, idx)
+    decreases |pt'|
+  {
+    if idx + 1 == NumBuckets(pt) {
+    } else {
+      TranslatePivotsCondition(pt, prefix, newPrefix, end, idx+1, pt'[1..]);
+    }
+  }
+
+  method ComputeTranslatePivots(pt: PivotTable, prefix: Key, newPrefix: Key, end: Element) returns (pt': PivotTable)
+  requires |pt| < Uint64UpperBound()
+  requires WFPivots(pt)
+  requires forall i | 0 <= i < NumBuckets(pt) :: IsPrefix(prefix, pt[i].e)
+  requires end.Element? ==> ElementIsKey(end)
+  requires Keyspace.lt(TranslateElement(pt[|pt|-2], prefix, newPrefix), end)
+  ensures pt' == TranslatePivots(pt, prefix, newPrefix, end, 0)
+  {
+    linear var result := seq_alloc_init(|pt| as uint64, end);
+
+    var i := 0;
+    while i < |pt| as uint64 - 1
+      invariant 0 <= i <= |pt| as uint64 - 1
+      invariant |result| == |pt|
+      invariant forall j | 0 <= j < i :: result[j] == TranslateElement(pt[j], prefix, newPrefix)
+      invariant Last(result) == end
+    {
+      var tmp := ComputeTranslateElement(pt[i], prefix, newPrefix);
+      mut_seq_set(inout result, i, tmp);
+      i := i + 1;
+    }
+    pt' := seq_unleash(result);
+    TranslatePivotsCondition(pt, prefix, newPrefix, end, 0, pt');
+  }
+
+  lemma TranslateEdgesCondition(et: EdgeTable, pt: PivotTable, idx: int, et': EdgeTable)
+    requires TranslateEdges.requires(et, pt, idx)
+    requires |et'| == |et| - idx
+    requires forall i | 0 <= i < |et'| :: et'[i] == if et[idx + i].Some? then et[idx + i] else Some(PivotLcp(pt[idx + i], pt[idx + i +1]))
+    ensures et' == TranslateEdges(et, pt, idx)
+    decreases |et'|
+  {
+  }
+
+  method ComputeTranslateEdges(et: EdgeTable, pt: PivotTable) returns (et': EdgeTable)
+  requires |et| < Uint64UpperBound()
+  requires WFPivots(pt)
+  requires WFEdges(et, pt)
+  ensures et' == TranslateEdges(et, pt, 0)
+  {
+    linear var result := seq_alloc(|et| as uint64, None);
+
+    var i := 0;
+    while i < |et| as uint64
+      invariant 0 <= i <= |et| as uint64
+      invariant |result| == |et|
+      invariant forall j | 0 <= j < i :: result[j] == if et[j].Some? then et[j] else Some(PivotLcp(pt[j], pt[j+1]));
+    {
+      if et[i].Some? {
+        mut_seq_set(inout result, i, et[i]);
+      } else {
+        var newPrefix := ComputePivotLcp(pt[i], pt[i+1]);
+        mut_seq_set(inout result, i, Some(newPrefix));
+      }
+      i := i + 1;
+    }
+    et' := seq_unleash(result);
+    TranslateEdgesCondition(et, pt, 0, et');
+  }
+
+  function {:opaque} TranslateBucketSimple(bucket: Bucket, prefix: Key, newPrefix: Key, i: nat) : (result: Bucket)
+    requires PreWFBucket(bucket)
+    requires 0 <= i <= |bucket.keys|
+    ensures |result.keys| <= i
+    ensures PreWFBucket(result)
+    ensures EncodableMessageSeq(bucket.msgs) ==> EncodableMessageSeq(result.msgs)
+    decreases i
+  {
+    if i == 0 then
+      EmptyBucket()
+    else if IsPrefix(prefix, bucket.keys[i - 1]) then
+      var prefixBucket := TranslateBucketSimple(bucket, prefix, newPrefix, i - 1);
+      var oldkey: seq<byte> := bucket.keys[i - 1];
+      assume |newPrefix + oldkey[|prefix|..]| <= 1024;
+      var newKey := newPrefix + oldkey[|prefix|..];
+      Bucket(prefixBucket.keys + [ newKey ], prefixBucket.msgs + [ bucket.msgs[i - 1] ])
+    else
+      TranslateBucketSimple(bucket, prefix, newPrefix, i - 1)
+  }
+
+  lemma TranslateBucketSimpleEquivalence(bucket: Bucket, prefix: Key, newPrefix: Key)
+    requires PreWFBucket(bucket)
+    ensures TranslateBucketSimple(bucket, prefix, newPrefix, |bucket.keys|) == TranslateBucket(bucket, prefix, newPrefix)
+
+  predicate {:opaque} WillFitInPkv(mbucket: MutBucket, prefix: Key, newPrefix: Key)
+    requires mbucket.Inv()
+  {
+    && PackedKV.PSA.psaCanAppendSeq(PackedKV.PSA.EmptyPsa(), TranslateBucket(mbucket.I(), prefix, newPrefix).keys)
+    && PackedKV.PSA.psaCanAppendSeq(PackedKV.PSA.EmptyPsa(), messageSeq_to_bytestringSeq(TranslateBucket(mbucket.I(), prefix, newPrefix).msgs))
+    && var psaKeys := PackedKV.PSA.psaFromSeq(TranslateBucket(mbucket.I(), prefix, newPrefix).keys);
+    && var psaMsgs := PackedKV.PSA.psaFromSeq(messageSeq_to_bytestringSeq(TranslateBucket(mbucket.I(), prefix, newPrefix).msgs));
+    && PackedKV.WeightPkv(PackedKV.Pkv(psaKeys, psaMsgs)) as nat < Uint32UpperBound()
+  }
+
+  predicate TranslateBucketWillFit(bucket: Bucket, prefix: Key, newPrefix: Key)
+  requires PreWFBucket(bucket)
+  {
+    (|newPrefix| <= |prefix| || |bucket.keys| * 1024 < 0x1_0000_0000)
+  }
+
+  predicate TranslateBucketsWillFit(buckets: seq<Bucket>, prefix: Key, newPrefix: Key)
+  requires forall i | 0 <= i < |buckets| :: PreWFBucket(buckets[i])
+  {
+    (forall i | 0 <= i < |buckets| :: TranslateBucketWillFit(buckets[i], prefix, newPrefix))
+  }
+
+  method ComputeTranslateBucketWillFit(shared mbucket: MutBucket, prefix: Key, newPrefix: Key)
+  returns (b: bool)
+  requires mbucket.Inv()
+  ensures b == TranslateBucketWillFit(mbucket.I(), prefix, newPrefix)
+  ensures b ==> WillFitInPkv(mbucket, prefix, newPrefix)
+  {
+    if |newPrefix| <= |prefix| {
+      b := true;
+    } else {
+      // TODO: do different key length calculation based on format of bucket
+      var pkv := mbucket.GetPkv();
+      var size := PackedKV.NumKVPairs(pkv);
+      b := size * 1024 < 0x1_0000_0000;
+    }
+    TranslateBucketWillFitImpliesWillFitInPkv(mbucket, prefix, newPrefix);
+  }
+
+  method ComputeTranslateBucketsWillFit(shared mbuckets: lseq<MutBucket>, prefix: Key, newPrefix: Key)
+  returns (b: bool)
+  requires MutBucket.InvLseq(mbuckets)
+  ensures b == TranslateBucketsWillFit(MutBucket.ILseq(mbuckets), prefix, newPrefix)
+  ensures b ==> (forall i | 0 <= i < |mbuckets| :: WillFitInPkv(lseqs(mbuckets)[i], prefix, newPrefix))
+  {
+    var i := 0;
+    b := true;
+
+    while i < lseq_length_as_uint64(mbuckets)
+      invariant 0 <= i <= |mbuckets| as uint64
+      invariant forall j | 0 <= j < i :: TranslateBucketWillFit(lseqs(mbuckets)[j].I(), prefix, newPrefix)
+      invariant forall j | 0 <= j < i :: WillFitInPkv(lseqs(mbuckets)[j], prefix, newPrefix)
+    {
+      b := ComputeTranslateBucketWillFit(lseq_peek(mbuckets, i), prefix, newPrefix);
+      if !b {
+        return false;
+      }
+      i := i + 1;
+    }
+  }
+
+  lemma TranslateBucketWillFitImpliesWillFitInPkv(mbucket: MutBucket, prefix: Key, newPrefix: Key)
+  requires mbucket.Inv()
+  ensures TranslateBucketWillFit(mbucket.I(), prefix, newPrefix) ==> WillFitInPkv(mbucket, prefix, newPrefix)
+  {
+    // 
+    assume false;
+    var b := mbucket.I();
+    var tb := TranslateBucket(b, prefix, newPrefix);
+    var idxs := TranslateBucketInternal(b, prefix, newPrefix, 0).idxs;
+  
+    if mbucket.format.BFTree? {
+      var tree := mbucket.format.tree;
+      var treekeys := LKMB.Model.ToSeq(tree).0;
+      var treemsgs := LKMB.Model.ToSeq(tree).1;
+
+      LKMBPKVOps.ToSeqInterpretation(tree);
+      LKMB.Model.ToSeqIsStrictlySorted(tree);
+      assert Bucket(treekeys, treemsgs).as_map() == b.as_map();
+      assert Lexi.IsStrictlySorted(treekeys);
+      assert Lexi.IsStrictlySorted(b.keys);
+
+      MapSeqs.SeqsEqOfMapsEq(treekeys, treemsgs, b.keys, b.msgs);
+      assert b.keys == treekeys;
+      assert b.msgs == treemsgs;
+
+      LKMBPKVOps.WeightImpliesCanAppend(tree);
+    } else {
+      var pkv := mbucket.format.pkv;
+      assert PackedKV.WF(pkv);
+      assert b == PackedKV.I(pkv);
+
+      assert PackedKV.PSA.I(pkv.keys) == b.keys;
+      assert PackedKV.PSA.I(pkv.messages) == messageSeq_to_bytestringSeq(b.msgs);
+
+      PackedKV.PSA.psaCanAppendI(pkv.keys);
+      PackedKV.PSA.psaCanAppendI(pkv.messages);
+    }
+
+    assert EncodableMessageSeq(b.msgs);
+    assert PackedKV.PSA.psaCanAppendSeq(PackedKV.PSA.EmptyPsa(), b.keys);
+    assert PackedKV.PSA.psaCanAppendSeq(PackedKV.PSA.EmptyPsa(), messageSeq_to_bytestringSeq(b.msgs));
+
+    if |newPrefix| <= |prefix| {
+      TranslateBucketKeyLt(b, tb, idxs, prefix, newPrefix);
+    } else if |b.keys| * 1024 < 0x1_0000_0000 {
+      FlattenLengthUpperBound(FlattenShape(tb.keys));
+      assert PackedKV.PSA.psaCanAppendSeq(PackedKV.PSA.EmptyPsa(), tb.keys);
+    }
+
+    TranslateBucketMessageLt(b, tb, idxs, prefix, newPrefix);
+    assert PackedKV.PSA.psaCanAppendSeq(PackedKV.PSA.EmptyPsa(), messageSeq_to_bytestringSeq(tb.msgs));
+
+    reveal_WillFitInPkv();
+  }
+
+  lemma FlattenLengthUpperBound(len: seq<nat>)
+  requires forall i | 0 <= i < |len| :: len[i] <= 1024
+  ensures FlattenLength(len) <= |len| * 1024
+  decreases |len|
+  {
+    reveal_FlattenLength();
+
+    if |len| > 0 {
+      FlattenLengthUpperBound(len[1..]);
+      FlattenLengthAdditive([len[0]], len[1..]);
+      assert [len[0]] + len[1..] == len;
+    }
+  }
+
+  lemma TranslateBucketKeyLt(bucket: Bucket, bucket': Bucket, idxs: seq<int>, prefix: Key, newPrefix: Key)
+  requires WFBucket(bucket)
+  requires |newPrefix| <= |prefix|
+  requires WFTBucket(bucket, TBucket(bucket', idxs), prefix, newPrefix, 0)
+  ensures FlattenLength(FlattenShape(bucket'.keys)) <= FlattenLength(FlattenShape(bucket.keys))
+  {
+    reveal_WFTBucket();
+    var keylen := FlattenShape(bucket.keys);
+    var keylen' := FlattenShape(bucket'.keys);
+
+    TranslateBucketFlattenLengthLt(keylen, keylen', idxs);
+    if |idxs| > 0 {
+      FlattenLengthSubSeq(keylen, idxs[0], |keylen|);
+      assert keylen[idxs[0]..] == keylen[idxs[0]..|keylen|];
+    }
+  }
+
+  lemma TranslateBucketMessageLt(bucket: Bucket, bucket': Bucket, idxs: seq<int>, prefix: Key, newPrefix: Key)
+  requires WFBucket(bucket)
+  requires WFTBucket(bucket, TBucket(bucket', idxs), prefix, newPrefix, 0)
+  ensures EncodableMessageSeq(bucket'.msgs)
+  ensures FlattenLength(FlattenShape(messageSeq_to_bytestringSeq(bucket'.msgs)))
+     <= FlattenLength(FlattenShape(messageSeq_to_bytestringSeq(bucket.msgs)))
+  {
+    reveal_WFTBucket();
+
+    var msglen := FlattenShape(messageSeq_to_bytestringSeq(bucket.msgs));
+    var msglen' := FlattenShape(messageSeq_to_bytestringSeq(bucket'.msgs));
+
+    TranslateBucketFlattenLengthLt(msglen, msglen', idxs);
+    if |idxs| > 0 {
+      FlattenLengthSubSeq(msglen, idxs[0], |msglen|);
+      assert msglen[idxs[0]..] == msglen[idxs[0]..|msglen|];
+    }
+  }
+
+  lemma TranslateBucketFlattenLengthLt(len: seq<nat>, len': seq<nat>, idxs: seq<int>)
+  requires |idxs| == |len'| <= |len|
+  requires forall i | 0 <= i < |idxs| :: 0 <= idxs[i] < |len|
+  requires forall i | 0 <= i < |idxs| :: len[idxs[i]] >= len'[i]
+  requires forall i, j | 0 <= i < j < |idxs| :: idxs[i] < idxs[j]
+  ensures |idxs| > 0 ==> FlattenLength(len') <= FlattenLength(len[idxs[0]..])
+  ensures |idxs| == 0 ==> FlattenLength(len') == 0
+  decreases |idxs|
+  {
+    reveal_FlattenLength();
+
+    if |len'| > 0 {
+      var i := idxs[0];
+      TranslateBucketFlattenLengthLt(len, len'[1..], idxs[1..]);
+
+      FlattenLengthAdditive([len'[0]], len'[1..]);
+      FlattenLengthAdditive([len[i]], len[i+1..]);
+      assert [len'[0]] + len'[1..] == len';
+      assert [len[i]] + len[i+1..] == len[i..];
+
+      if |idxs| > 1{
+        FlattenLengthAdditive([len[i]], len[i+1..idxs[1]]);
+        FlattenLengthAdditive(len[i..idxs[1]], len[idxs[1]..]);
+        assert [len[i]] + len[i+1..idxs[1]] == len[i..idxs[1]];
+        assert len[i..idxs[1]] + len[idxs[1]..] == len[i..];
+      }
+    }
+  }
+
+  lemma SplitLeftWillFitInPkv(bucket: MutBucket, bucket': MutBucket, prefix: Key, newPrefix: Key, pivot: Key)
+  requires bucket.Inv()
+  requires bucket'.Inv()
+  requires bucket'.I() == SplitBucketLeft(bucket.I(), pivot)
+  ensures WillFitInPkv(bucket, prefix, newPrefix) ==> WillFitInPkv(bucket', prefix, newPrefix)
+  {
+    assume false;
+  }
+
+  lemma SplitRightWillFitInPkv(bucket: MutBucket, bucket': MutBucket, prefix: Key, newPrefix: Key, pivot: Key)
+  requires bucket.Inv()
+  requires bucket'.Inv()
+  requires bucket'.I() == SplitBucketRight(bucket.I(), pivot)
+  ensures WillFitInPkv(bucket, prefix, newPrefix) ==> WillFitInPkv(bucket', prefix, newPrefix)
+  {
+    assume false;
+  }
+  
+  method ComputeTranslateBucket(shared mbucket: MutBucket, prefix: Key, newPrefix: Key) returns (linear mbucket': MutBucket)
+  requires mbucket.Inv()
+  requires WillFitInPkv(mbucket, prefix, newPrefix);
+  ensures mbucket'.Inv()
+  ensures mbucket'.I() == TranslateBucket(mbucket.I(), prefix, newPrefix)
+  {
+    reveal_WillFitInPkv();
+    ghost var bucket := mbucket.I();
+    assert EncodableMessageSeq(bucket.msgs);
+    TranslateBucketSimpleEquivalence(bucket, prefix, newPrefix);
+    reveal_IsPrefix();
+
+    var pkv := mbucket.GetPkv();
+    var len := PackedKV.NumKVPairs(pkv);
+    linear var result_keys := seq_alloc_init(len, []);
+    linear var result_msgs := seq_alloc_init(len, []);
+    var result_len := 0;
+
+    var i := 0;
+    while i < len
+      invariant 0 <= i <= len
+      invariant 0 <= result_len <= i
+      invariant |result_keys| == len as nat
+      invariant |result_msgs| == len as nat
+      invariant result_keys[..result_len] == TranslateBucketSimple(bucket, prefix, newPrefix, i as nat).keys
+      invariant forall j | 0 <= j < result_len :: |result_msgs[j]| < 0x1_0000_0000
+      invariant result_msgs[..result_len] == messageSeq_to_bytestringSeq(TranslateBucketSimple(bucket, prefix, newPrefix, i as nat).msgs)
+    {
+      var key: seq<byte> := PackedKV.GetKey(pkv, i);
+      var msg := PackedKV.PSA.psaElement(pkv.messages, i);
+      if |prefix| as uint64 <= |key| as uint64 && prefix == key[..|prefix| as uint64] {
+        assume |newPrefix + key[|prefix| as uint64..]| <= 1024;
+        mut_seq_set(inout result_keys, result_len, newPrefix + key[|prefix| as uint64..]);
+        mut_seq_set(inout result_msgs, result_len, msg);
+        result_len := result_len + 1;
+        calc {
+          result_keys[..result_len];
+          { reveal_TranslateBucketSimple(); }
+          TranslateBucketSimple(bucket, prefix, newPrefix, i as nat + 1).keys;
+        }
+        calc {
+          result_msgs[..result_len];
+          // result_msgs[..result_len-1] + [result_msgs[result_len-1]];
+          // messageSeq_to_bytestringSeq(TranslateBucketSimple(bucket, prefix, newPrefix, i as nat).msgs) + [result_msgs[result_len-1]];
+          // messageSeq_to_bytestringSeq(TranslateBucketSimple(bucket, prefix, newPrefix, i as nat).msgs) + [PackedKV.PSA.psaElement(pkv.messages, i)];
+          messageSeq_to_bytestringSeq(TranslateBucketSimple(bucket, prefix, newPrefix, i as nat).msgs) + [PackedKV.PSA.I(pkv.messages)[i]];
+          // messageSeq_to_bytestringSeq(TranslateBucketSimple(bucket, prefix, newPrefix, i as nat).msgs) + [Message_to_bytestring(bucket.msgs[i])];
+          // messageSeq_to_bytestringSeq(TranslateBucketSimple(bucket, prefix, newPrefix, i as nat).msgs) + messageSeq_to_bytestringSeq([bucket.msgs[i]]);
+          { messageSeq_to_bytestringSeq_Additive(TranslateBucketSimple(bucket, prefix, newPrefix, i as nat).msgs, [bucket.msgs[i]]); }
+          messageSeq_to_bytestringSeq(TranslateBucketSimple(bucket, prefix, newPrefix, i as nat).msgs + [bucket.msgs[i]]);
+          { reveal_TranslateBucketSimple(); }
+          messageSeq_to_bytestringSeq(TranslateBucketSimple(bucket, prefix, newPrefix, i as nat + 1).msgs);
+        }
+      } else {
+        reveal_TranslateBucketSimple();
+      }
+      i := i + 1;
+    }
+
+    assume false;
+
+    var result_keys' := seq_unleash(result_keys);
+    var result_msgs' := seq_unleash(result_msgs);
+
+    assert result_keys'[..result_len] == TranslateBucket(mbucket.I(), prefix, newPrefix).keys;
+    //assert result_msgs'[..result_len] == messageSeq_to_bytestringSeq(TranslateBucket(mbucket.I(), prefix, newPrefix).msgs);
+    var result_keys_psa := PackedKV.PSA.FromSeq(result_keys'[..result_len]);
+    var result_msgs_psa := PackedKV.PSA.FromSeq(result_msgs'[..result_len]);
+    calc {
+      result_keys_psa;
+      { PackedKV.PSA.psaCanAppendI(result_keys_psa); }
+    //   PackedKV.PSA.psaFromSeq(result_keys'[..result_len]);
+    //   PackedKV.PSA.psaFromSeq(TranslateBucketSimple(bucket, prefix, newPrefix, i as nat).keys);
+    //   PackedKV.PSA.psaFromSeq(TranslateBucket(bucket, prefix, newPrefix).keys);
+      PackedKV.PSA.psaFromSeq(TranslateBucket(mbucket.I(), prefix, newPrefix).keys);
+    }
+    calc {
+      result_msgs_psa;
+      { PackedKV.PSA.psaCanAppendI(result_msgs_psa); }
+    //   PackedKV.PSA.psaFromSeq(result_msgs'[..result_len]);
+    //   PackedKV.PSA.psaFromSeq(messageSeq_to_bytestringSeq(TranslateBucketSimple(bucket, prefix, newPrefix, i as nat).msgs));
+    //   PackedKV.PSA.psaFromSeq(messageSeq_to_bytestringSeq(TranslateBucket(bucket, prefix, newPrefix).msgs));
+      PackedKV.PSA.psaFromSeq(messageSeq_to_bytestringSeq(TranslateBucket(mbucket.I(), prefix, newPrefix).msgs));
+    }
+    mbucket' := MutBucket.AllocPkv(PackedKV.Pkv(result_keys_psa, result_msgs_psa), mbucket.sorted);
+  }
+
+  // method ComputeTranslateBuckets(shared blist: lseq<MutBucket>, prefix: Key, newPrefix: Key) returns (linear blist': lseq<MutBucket>)
+  // requires MutBucket.InvLseq(blist)
+  // requires forall i | 0 <= i < |blist| :: WillFitInPkv(blist[i], prefix, newPrefix)
+  // ensures MutBucket.InvLseq(blist')
+  // ensures MutBucket.ILseq(blist') == TranslateBuckets(MutBucket.ILseq(blist), prefix, newPrefix)
+  // {
+  //   ghost var iblist := MutBucket.ILseq(blist);
+
+  //   blist' := lseq_alloc(lseq_length_as_uint64(blist));
+
+  //   var i := 0;
+  //   while i < lseq_length_as_uint64(blist)
+  //     invariant 0 <= i <= |blist| as uint64
+  //     invariant |blist'| == |blist|
+  //     invariant forall j | 0 <= j < |blist| as uint64 :: lseq_has(blist')[j] <==> (j < i)
+  //     invariant MutBucket.InvSeq(lseqs(blist')[..i])
+  //     invariant MutBucket.ISeq(lseqs(blist')[..i]) == TranslateBuckets(iblist[..i], prefix, newPrefix)
+  //   {
+  //     linear var tmp := ComputeTranslateBucket(lseq_peek(blist, i), prefix, newPrefix);
+  //     lseq_give_inout(inout blist', i, tmp);
+  //     i := i + 1;
+
+  //     assert lseqs(blist')[..i] == lseqs(blist')[..i-1] + [lseqs(blist')[i-1]];
+  //   }
+  //   assert lseqs(blist') == lseqs(blist')[..i];
+  //   assert iblist == iblist[..i];
+  // }
+
+  method ComputeTranslateSingleBucketList(linear bucket: MutBucket, prefix: Key, newPrefix: Key)
+  returns (linear blist: lseq<MutBucket>)
+  requires bucket.Inv()
+  requires WillFitInPkv(bucket, prefix, newPrefix)
+  ensures MutBucket.InvLseq(blist)
+  ensures MutBucket.ILseq(blist) == TranslateBuckets([bucket.I()], prefix, newPrefix)
+  {
+    blist := lseq_alloc(1);
+    linear var tbucket := ComputeTranslateBucket(bucket, prefix, newPrefix);
+    lseq_give_inout(inout blist, 0, tbucket);
+    assert MutBucket.ILseq(blist) == TranslateBuckets([bucket.I()], prefix, newPrefix);
+    var _ := FreeMutBucket(bucket);
+  }
+
+  method ComputeTranslateCutOffKeepRightBuckets(shared blist: lseq<MutBucket>, linear bucket: MutBucket, 
+    prefix: Key, newPrefix: Key, cRight: uint64) returns (linear blist': lseq<MutBucket>)
+  requires bucket.Inv()
+  requires MutBucket.InvLseq(blist)
+  requires WillFitInPkv(bucket, prefix, newPrefix)
+  requires forall i | 0 <= i < |blist| :: WillFitInPkv(blist[i], prefix, newPrefix)
+  requires 0 <= cRight as int < |blist|
+  requires |blist| < 0x1_0000_0000_0000_0000
+  ensures MutBucket.InvLseq(blist')
+  ensures MutBucket.ILseq(blist') == TranslateBuckets([bucket.I()]+ MutBucket.ILseq(blist)[cRight+1..], prefix, newPrefix)
+  {
+    ghost var iblist := [bucket.I()] + MutBucket.ILseq(blist)[cRight+1..];
+    blist' := lseq_alloc(lseq_length_as_uint64(blist)-cRight);
+
+    linear var b := ComputeTranslateBucket(bucket, prefix, newPrefix);
+    lseq_give_inout(inout blist', 0, b);
+    var _ := FreeMutBucket(bucket);
+
+    var i := 1;
+    while i < lseq_length_as_uint64(blist')
+      invariant 1 <= i as int <= |blist'|
+      invariant |blist'| == |iblist|
+      invariant |blist'| + cRight as int == |blist|
+      invariant forall j | 0 as int <= j < |blist| :: lseq_has(blist)[j]
+      invariant forall j | 0 as int <= j < |blist| :: lseqs(blist)[j].Inv()
+      invariant forall j | 1 <= j < |iblist| :: iblist[j] == lseqs(blist)[j+cRight as int].I()
+      invariant forall j | 0 <= j < |blist'| :: lseq_has(blist')[j] <==> j < i as int
+      invariant forall j | 0 <= j < i :: lseqs(blist')[j].Inv()   
+      invariant forall j | 0 <= j < i :: lseqs(blist')[j].I() == TranslateBucket(iblist[j], prefix, newPrefix)
+    {
+      linear var tmp := ComputeTranslateBucket(lseq_peek(blist, i+cRight), prefix, newPrefix);
+      assert lseqs(blist)[i+cRight].I() == iblist[i];
+      assert tmp.I() == TranslateBucket(iblist[i], prefix, newPrefix);
+
+      lseq_give_inout(inout blist', i, tmp);
+      i := i + 1;
+    }
+  }
+
+  method ComputeTranslateCutOffNodeBuckets(shared blist: lseq<MutBucket>, linear left: MutBucket, linear right: MutBucket,
+    prefix: Key, newPrefix: Key, cLeft: uint64, cRight: uint64) returns (linear blist': lseq<MutBucket>)
+  requires left.Inv()
+  requires right.Inv()
+  requires MutBucket.InvLseq(blist)
+  requires 0 <= cRight as int < cLeft as int < |blist|
+  requires WillFitInPkv(left, prefix, newPrefix)
+  requires WillFitInPkv(right, prefix, newPrefix)
+  requires forall i | cRight as int+1 <= i < cLeft as int :: WillFitInPkv(blist[i], prefix, newPrefix)
+  requires |blist| < 0x1_0000_0000_0000_0000
+  ensures MutBucket.InvLseq(blist')
+  ensures MutBucket.ILseq(blist') == 
+    TranslateBuckets([left.I()]+ MutBucket.ILseq(blist)[cRight+1..cLeft] + [right.I()], prefix, newPrefix) 
+  {
+    ghost var iblist := [left.I()] + MutBucket.ILseq(blist)[cRight+1..cLeft] + [right.I()];
+    blist' := lseq_alloc(cLeft-cRight+1);
+
+    linear var b1 := ComputeTranslateBucket(left, prefix, newPrefix);
+    lseq_give_inout(inout blist', 0, b1);
+    var _ := FreeMutBucket(left);
+
+    var i := 1;
+    while i < lseq_length_as_uint64(blist')-1
+      invariant 1 <= i as int < |blist'|
+      invariant |blist'| == |iblist|
+      invariant |blist'| == cLeft as int - cRight as int +1
+      invariant forall j | 0 as int <= j < |blist| :: lseq_has(blist)[j]
+      invariant forall j | 0 as int <= j < |blist| :: lseqs(blist)[j].Inv()
+      invariant forall j | 1 <= j < |iblist|-1 :: iblist[j] == lseqs(blist)[j+cRight as int].I()
+      invariant forall j | 0 <= j < |blist'| :: lseq_has(blist')[j] <==> j < i as int
+      invariant forall j | 0 <= j < i :: lseqs(blist')[j].Inv()   
+      invariant forall j | 0 <= j < i :: lseqs(blist')[j].I() == TranslateBucket(iblist[j], prefix, newPrefix)
+    {
+      linear var tmp := ComputeTranslateBucket(lseq_peek(blist, i+cRight), prefix, newPrefix);
+      assert tmp.I() == TranslateBucket(iblist[i], prefix, newPrefix);
+
+      lseq_give_inout(inout blist', i, tmp);
+      i := i + 1;
+    }
+
+    linear var b2 := ComputeTranslateBucket(right, prefix, newPrefix);
+    lseq_give_inout(inout blist', i, b2);
+    var _ := FreeMutBucket(right);
+  }
+
+  method ComputeParentKeysInChildRange(parentpivots: PivotTable, parentedges: EdgeTable, childpivots: PivotTable, slot: uint64)
+  returns (b: bool)
+  requires WFPivots(parentpivots)
+  requires WFPivots(childpivots)
+  requires WFEdges(parentedges, parentpivots)
+  requires 0 <= slot as int < |parentedges|
+  requires |parentpivots| < Uint64UpperBound()
+  requires |childpivots| < 0x4000_0000_0000_0000
+  ensures b == ParentKeysInChildRange(parentpivots, parentedges, childpivots, slot as int)
+  {
+    Keyspace.reveal_IsStrictlySorted();
+    if parentedges[slot].None? {
+      b := ComputeContainsRange(childpivots, parentpivots[slot], parentpivots[slot+1]);
+    } else {
+      var prefix := ComputePivotLcp(parentpivots[slot], parentpivots[slot + 1]);
+      var newPrefix := parentedges[slot].value;
+      var left, right := ComputeTranslatePivotPair(parentpivots[slot].e, parentpivots[slot + 1], prefix, newPrefix);
+      b := ComputeContainsRange(childpivots, Keyspace.Element(left), right);
+    }
+  }
+}
